dataset/MBPP-DFY-50/dfy_files/task_id_131.dfy
@@ -1,0 +1,40 @@
+predicate IsVowel(c: char)
+{
+    c in {'a', 'e', 'i', 'o', 'u', 'A', 'E', 'I', 'O', 'U'}
+}
+
+method ReverseVowels(s: string) returns (v: string)
+    ensures |v| == |s|
+    ensures forall i :: 0 <= i < |s| ==> (IsVowel(s[i]) ==> s[i] in v && v[i] in s && v[i] != s[i]) && (!IsVowel(s[i]) ==> v[i] == s[i])
+{
+    var vowels : seq<char> := [];
+    for i := 0 to |s|
+    invariant 0 <= i <= |s|
+    invariant forall k :: 0 <= k < i && IsVowel(s[k]) ==> s[k] in vowels
+    {
+        if IsVowel(s[i])
+        {
+            vowels := [s[i]] + vowels;
+        }
+    }
+
+    var j := 0;
+    var s' : string := [];
+    for i := 0 to |s|
+    invariant 0 <= i <= |s|
+    invariant |s'| == i
+    invariant forall k :: 0 <= k < i && IsVowel(s[k]) ==> s'[k] in vowels
+    invariant forall k :: 0 <= k < i && !IsVowel(s[k]) ==> s[k] == s'[k]
+    {
+        if IsVowel(s[i])
+        {
+            s' := s' + [vowels[j]];
+            j := j + 1;
+        }
+        else 
+        {
+            s' := s' + [s[i]];
+        }
+    }
+    return s';
+}
