dataset/MBPP-DFY-50/dfy_files/task_id_167.dfy
@@ -1,0 +1,14 @@
+method SmallestPowerOfTwo(n: int) returns (power: int)
+    requires n > 0
+    ensures power >= n && exists k :: power == 2^k
+    ensures forall k :: (2^k < n) ==> power != 2^k
+{
+    power := 1;
+    while power < n
+        invariant power > 0
+        invariant exists k :: power == 2^k
+        invariant forall k :: (2^k < n) ==> power != 2^k
+    {
+        power := power * 2;
+    }
+}
