dataset/MBPP-DFY-50/dfy_files/task_id_256.dfy
@@ -1,0 +1,35 @@
+predicate IsPrime(n: int)
+    {
+        if n < 2 then false
+        else if n == 2 then true
+        else if n % 2 == 0 then false
+        else {
+            var i := 3;
+            while (i * i <= n)
+                invariant 2 <= i
+                invariant (forall k :: 2 <= k < i ==> n % k != 0)
+            {
+                if n % i == 0 then return false;
+                i := i + 2;
+            }
+            true
+        }
+    }
+
+    method CountPrimes(n: int) returns (count: int)
+    requires n >= 0
+    ensures count >= 0
+    ensures count == | set i: int | 2 <= i < n && IsPrime(i)|
+{
+    count := 0;
+    var i := 2;
+    while i < n
+        invariant 2 <= i <= n
+        invariant count == | set k: int | 2 <= k < i && IsPrime(k)|
+    {
+        if IsPrime(i) {
+            count := count + 1;
+        }
+        i := i + 1;
+    }
+}
