dataset/MBPP-DFY-50/dfy_files/task_id_420.dfy
@@ -1,0 +1,15 @@
+method CubeSumOfEvenNumbers(n: int) returns (sum: int)
+    requires n >= 0
+    ensures sum == n * n * (n + 1) * (n + 1)
+{
+    sum := 0;
+    var i := 0;
+    for k := 0 to n
+        invariant 0 <= k <= n
+        invariant i == 2 * k
+        invariant sum == k * k * (k + 1) * (k + 1)
+    {
+        sum := sum + i * i * i;
+        i := i + 2;
+    }
+}
