dataset/MBPP-DFY-50/dfy_files/task_id_448.dfy
@@ -1,0 +1,26 @@
+function perrin(n: int): int
+    requires n >= 0
+    decreases n
+    {
+        if n < 3 then n else perrin(n - 2) + perrin(n - 3)
+    }
+
+    method PerrinSum(n: int) returns (sum: int)
+    requires n >= 0
+    ensures sum == sumPerrin(n)
+    {
+        sum := 0;
+        for i := 0 to n
+            invariant 0 <= i <= n
+            invariant sum == sumPerrin(i)
+        {
+            sum := sum + perrin(i);
+        }
+    }
+
+    function sumPerrin(n: int): int
+    requires n >= 0
+    decreases n
+    {
+        if n == 0 then 0 else perrin(n) + sumPerrin(n - 1)
+    }
