dataset/MBPP-DFY-50/dfy_files/task_id_559.dfy
@@ -1,0 +1,30 @@
+method MaxSubArraySum(a: array<int>) returns (maxSum: int)
+    requires a.Length > 0
+    ensures maxSum >= a[Max(a[..])]
+    ensures exists i, j :: 0 <= i <= j < a.Length && maxSum == Sum(a[i..j+1])
+{
+    var currentSum := a[0];
+    maxSum := a[0];
+
+    for i := 1 to a.Length
+        invariant 0 <= i <= a.Length
+        invariant maxSum >= a[Max(a[..i])]
+        invariant exists k, l :: 0 <= k <= l < i && maxSum == Sum(a[k..l+1])
+    {
+        currentSum := Max(currentSum + a[i], a[i]);
+        maxSum := Max(maxSum, currentSum);
+    }
+}
+
+function Max(a: seq<int>): int
+    requires |a| > 0
+{
+    if |a| == 1 then a[0]
+    else Max(a[..|a|-1]) >? a[|a|-1]
+}
+
+function Sum(a: seq<int>): int
+{
+    if |a| == 0 then 0
+    else a[0] + Sum(a[1..])
+}
