dataset/MBPP-DFY-50/dfy_files/task_id_639.dfy
@@ -1,0 +1,20 @@
+predicate IsUpperCase(s: string)
+    requires |s| > 0
+    {
+        65 <= s[0] as int <= 90
+    }
+
+    method SumLengthOfNames(names: seq<string>) returns (sum: int)
+    requires names != null
+    ensures sum >= 0
+    ensures sum == | set n: string | n in names && IsUpperCase(n) | 
+    {
+        var filteredNames := set n: string | n in names && IsUpperCase(n);
+        sum := 0;
+        for n in filteredNames
+            invariant sum >= 0
+            invariant sum <= |filteredNames|
+        {
+            sum := sum + |n|;
+        }
+    }
