dataset/MBPP-DFY-50/dfy_files/task_id_67.dfy
@@ -1,0 +1,16 @@
+method BellNumber(n: nat) returns (bell: int)
+    requires n >= 0
+    ensures bell >= 0
+{
+    var bellNumbers := new int[n+1, n+1];
+    bellNumbers[0, 0] := 1;
+    for i := 1 to n+1
+    {
+        bellNumbers[i, 0] := bellNumbers[i-1, i-1];
+        for j := 1 to i
+        {
+            bellNumbers[i, j] := bellNumbers[i-1, j-1] + bellNumbers[i, j-1];
+        }
+    }
+    bell := bellNumbers[n, 0];
+}
