dataset/MBPP-DFY-50/dfy_files/task_id_806.dfy
@@ -1,0 +1,29 @@
+predicate IsUpperCase(c: char)
+{
+    65 <= c as int <= 90
+}
+
+method MaxRunUppercase(s: string) returns (maxRun: int)
+    ensures maxRun >= 0
+    ensures (exists i, j :: 0 <= i < j <= |s| && (forall k :: i <= k < j ==> IsUpperCase(s[k])) && j - i == maxRun) || (maxRun == 0 && forall i :: 0 <= i < |s| ==> !IsUpperCase(s[i]))
+{
+    var currentRun := 0;
+    maxRun := 0;
+
+    for i := 0 to |s|
+        invariant 0 <= i <= |s|
+        invariant 0 <= currentRun <= i
+        invariant (exists ii, jj :: 0 <= ii < jj <= i && (forall k :: ii <= k < jj ==> IsUpperCase(s[k])) && jj - ii == maxRun) || (maxRun == 0 && forall ii :: 0 <= ii < i ==> !IsUpperCase(s[ii]))
+
+    {
+        if IsUpperCase(s[i]) {
+            currentRun := currentRun + 1;
+            if currentRun > maxRun {
+                maxRun := currentRun;
+            }
+        }
+        else {
+            currentRun := 0;
+        }
+    }
+}
