dataset/MBPP-DFY-50/dfy_files/task_id_9.dfy
@@ -1,0 +1,38 @@
+method MinRotations(s: string) returns (rotations: int)
+    requires |s| > 0
+    ensures 0 <= rotations <= |s|
+    ensures (rotations == 0) <==> (forall i :: 0 < i < |s| ==> s != RotateRight(s, i))
+    ensures rotations > 0 ==> s == RotateRight(s, rotations)
+{
+    rotations := 0;
+    var temp: string;
+
+    for i := 1 to |s|
+        invariant 0 <= i <= |s|
+        invariant 0 <= rotations <= i
+        invariant (rotations == 0) <==> (forall k :: 0 < k < i ==> s != RotateRight(s, k))
+        invariant rotations > 0 ==> s == RotateRight(s, rotations)
+    {
+        temp := RotateRight(s, i);
+        if temp == s {
+            rotations := i;
+            break;
+        }
+    }
+}
+
+method RotateRight(s: string, n: int) returns (r: string)
+    requires n >= 0
+    ensures |r| == |s|
+    ensures forall i :: 0 <= i < |s| ==> r[i] == s[(i - n + |s|) % |s|]
+{
+    var rotated: string := "";
+    for i := 0 to |s|
+        invariant 0 <= i <= |s|
+        invariant |rotated| == i
+        invariant forall k :: 0 <= k < i ==> rotated[k] == s[(k - n + |s|) % |s|]
+    {
+        rotated := rotated + s[(i - n + |s|) % |s|];
+    }
+    return rotated;
+}
