dataset/MBPP-DFY-50/src/task_id_579.dfy
@@ -1,7 +1,5 @@
 method DissimilarElements(a: array<int>, b: array<int>) returns (result: seq<int>)
-  
   ensures forall x :: x in result ==> (InArray(a, x) != InArray(b, x))
-  
   ensures forall i, j :: 0 <= i < j < |result| ==> result[i] != result[j]
 {
   var res: seq<int> := [];
